Add HumanEvalLean example

tests/lean/run/cbv1.lean
@@ -96,6 +96,7 @@ example : "a" ++ "a" = "aa" := by
   conv =>
     lhs
     cbv
+  rfl
 
 #check String.utf8EncodeChar.eq_1
 
@@ -153,3 +154,49 @@ example : 2 + 2 = 4 := by
   conv =>
     lhs
     cbv
+
+def IsSubseq (s₁ : String) (s₂ : String) : Prop :=
+  List.Sublist s₁.toList s₂.toList
+
+def vowels : List Char := ['a', 'e', 'i', 'o', 'u', 'A', 'E', 'I', 'O', 'U']
+
+def NoVowels (s : String) : Prop :=
+  List.all s.toList (· ∉ vowels)
+
+def MaximalFor [LE α] (P : ι → Prop) (f : ι → α) (x : ι) : Prop :=
+  -- Same as MaximalFor in Mathlib
+  P x ∧ ∀ y : ι, P y → f x ≤ f y → f y ≤ f x
+
+def RemoveVowelsIff (solution : String → String) : Prop :=
+    (s x : String) → (solution s = x) → MaximalFor (fun i => NoVowels i ∧ IsSubseq i s) (String.length) x
+
+def removeVowels (s : String) : String :=
+    String.ofList (s.toList.filter (· ∉ vowels))
+
+example : removeVowels "abcdef" = "bcdf" := by
+  conv =>
+    lhs
+    cbv
+  rfl
+
+example : removeVowels "abcdef\nghijklm" = "bcdf\nghjklm" := by
+  conv =>
+    lhs
+    cbv
+  rfl
+example : removeVowels "aaaaa" = "" := by
+  conv =>
+    lhs
+    cbv
+  rfl
+example : removeVowels "aaBAA" = "B" := by
+  conv =>
+    lhs
+    cbv
+  rfl
+
+example : removeVowels "zbcd" = "zbcd" := by
+  conv =>
+    lhs
+    cbv
+  rfl
